@prefix amalgame: <http://purl.org/vocabularies/amalgame#> .
@prefix evaluator:<http://purl.org/vocabularies/amalgame/evaluator#> .
@prefix     skos: <http://www.w3.org/2004/02/skos/core#> .
@prefix    align: <http://knowledgeweb.semanticweb.org/heterogeneity/alignment#> .
@prefix     prov: <http://www.w3.org/ns/prov#> .
@prefix      owl: <http://www.w3.org/2002/07/owl#> .
@prefix      rdf: <http://www.w3.org/1999/02/22-rdf-syntax-ns#> .
@prefix     rdfs: <http://www.w3.org/2000/01/rdf-schema#> .
@prefix     xsd: <http://www.w3.org/2001/XMLSchema#> .

amalgame:AlignmentStrategy
    a prov:Plan ;
    rdfs:label "alignment strategy"@en ;
    rdfs:comment "RDF representation of an alignment strategy that can be loaded and executed by Amalgame"@en.

amalgame:Entity
    rdfs:label "entity"@en ;
    rdfs:comment "Top class for all amalgame data entities, including mappings and vocabularies"@en ;
    rdfs:subClassOf prov:Entity .

amalgame:Process
    rdfs:label "process"@en ;
    rdfs:comment "Top class for all amalgame processes"@en ;
    rdfs:subClassOf prov:Activity .

amalgame:parameters
    a rdf:Property ;
    rdfs:domain amalgame:Process ;
    rdfs:range rdfs:Literal .

amalgame:Matcher
    rdfs:label "matcher"@en ;
    skos:definition "Component that creates a mapping given a source and target vocabulary"@en ;
    rdfs:subClassOf amalgame:Process .
amalgame:Partitioner
    rdfs:label "partitioner"@en ;
    rdfs:subClassOf amalgame:Process .
amalgame:Selecter
    rdfs:label "selecter"@en ;
    rdfs:subClassOf amalgame:Process .
amalgame:MultiInputComponent
    rdfs:label "multi-input operator"@en ;
    skos:definition "Component with multiple first-class inputs"@en ;
    rdfs:subClassOf amalgame:Process .
amalgame:SetOperator
    rdfs:label "set operator"@en ;
    skos:definition "Component that creates a mapping by combining the correspondences from a number of mappings"@en ;
    rdfs:subClassOf amalgame:MultiInputComponent .
amalgame:MappingPartitioner
    rdfs:label "partitioner"@en ;
    skos:definition "Component that creates subsets from an existing mapping"@en ;
    rdfs:subClassOf amalgame:Partitioner .
amalgame:MappingSelecter
    rdfs:label "selecter"@en ;
    skos:definition "Component that creates a new mapping by selecting a number of correspondences from an existing mapping"@en ;
    rdfs:subClassOf amalgame:Selecter .
amalgame:VocabPartitioner
    rdfs:label "partitioner"@en ;
    skos:definition "Component that creates subsets from an existing concept scheme"@en ;
    rdfs:subClassOf amalgame:Partitioner .
amalgame:VocabSelecter
    rdfs:label "selecter"@en ;
    skos:definition "Component that creates a new conceptScheme by selecting a number of concepts from an existing concept scheme"@en ;
    rdfs:subClassOf amalgame:Selecter .
amalgame:VirtualVocabSelecter rdfs:subClassOf amalgame:VocabSelecter .
amalgame:VirtualVocabPartitioner rdfs:subClassOf amalgame:VocabPartitioner .
amalgame:MaterializedVocabSelecter rdfs:subClassOf amalgame:VocabSelecter . # deprecated
amalgame:Merger
    rdfs:label "merger"@en ;
    skos:definition "Component that creates a mapping by mergin the correspondences from a number of mappings"@en ;
    rdfs:subClassOf amalgame:Process .

amalgame:includes
        rdfs:domain skos:ConceptScheme ;
        rdfs:range amalgame:AlignmentStrategy .
amalgame:input
	rdfs:domain prov:Activity ;
	rdfs:range amalgame:Entity ;
	rdfs:subPropertyOf prov:used.
amalgame:secondary_input
	rdfs:domain prov:Activity ;
	rdfs:range amalgame:Entity ;
	rdfs:subPropertyOf prov:used .
amalgame:wasGeneratedBy 
	a rdf:Property ;
	rdfs:domain amalgame:Entity ;
	rdfs:range prov:Activity ;
	rdfs:comment 'The subject can be generated by running the object'@en.
amalgame:selectedBy
	rdfs:domain amalgame:Entity ;
	rdfs:range prov:Activity ;
	rdfs:subPropertyOf amalgame:wasGeneratedBy.
amalgame:discardedBy
	rdfs:domain amalgame:Entity ;
	rdfs:range prov:Activity ;
	rdfs:subPropertyOf amalgame:wasGeneratedBy.
amalgame:undecidedBy
	rdfs:domain amalgame:Entity ;
	rdfs:range prov:Activity ;
	rdfs:subPropertyOf amalgame:wasGeneratedBy.
amalgame:evaluationOf
	rdfs:subPropertyOf prov:wasDerivedFrom.
amalgame:Mapping a rdfs:Class ;
	rdfs:subClassOf prov:Entity ;
	rdfs:label "Mapping Graph"@en ;
	rdfs:comment "The class of all Named Graphs in the repository containing correspondences."@en.

amalgame:ConceptScheme
	rdfs:subClassOf skos:ConceptScheme .
amalgame:VirtualConceptScheme
	rdfs:subClassOf amalgame:ConceptScheme .

amalgame:LoadedMapping a rdfs:Class ;
	rdfs:subClassOf amalgame:Mapping ;
	rdfs:label "Loaded Mapping Graph"@en ;
	rdfs:comment "An alignment loaded from file, e.g. not derived from another alignment"@en.

amalgame:DerivedMapping a rdfs:Class ;
	rdfs:subClassOf amalgame:Mapping ;
	rdfs:label "Derived Mapping Graph"@en ;
	rdfs:comment "An mapping derived from another mapping"@en.

amalgame:OverlapMapping a rdfs:Class;
	rdfs:subClassOf amalgame:DerivedMapping ;
	rdfs:label "Amalgame Overlap"@en ;
	rdfs:comment "A Named Graph that describes the overlap of one or more other named graphs, these constituents are denoted by the amalgame:member property."@en .

amalgame:SampleMapping a rdfs:Class;
	rdfs:subClassOf amalgame:DerivedMapping ;
	rdfs:label "Amalgame Sample"@en ;
	rdfs:comment "A Named Graph that describes a sample of another named graph, denoted by dcterms:source in the amalgame:provenance section."@en .

amalgame:ExportedMapping a rdfs:Class;
	rdfs:subClassOf amalgame:DerivedMapping ;
	rdfs:label "Amalgame Exported"@en ;
	rdfs:comment "A Named Graph that has been created by exporting another named graph into a new format. The source graph is recorded by dcterms:source in the amalgame:provenance section."@en .

amalgame:PartitionedMapping a rdfs:Class;
	rdfs:subClassOf amalgame:DerivedMapping ;
	rdfs:label "Amalgame Partitioned"@en ;
	rdfs:comment "A Named Graph that has been created by partitioning another named graph into one or more new graphs. The source graph is recorded by dcterms:source in the amalgame:provenance section."@en .

amalgame:EvaluatedMapping a rdfs:Class;
	rdfs:subClassOf amalgame:Mapping ;
	rdfs:label "Amalgame Evaluation Results"@en ;
	rdfs:comment "A Named Graph that has been created by manually evaluating another named graph into a new graph. The source graph is recorded by the amalgame:evaluationOf property."@en .

amalgame:SelectionMapping a rdfs:Class;
	rdfs:subClassOf amalgame:DerivedMapping ;
	rdfs:label "Amalgame Selection Results"@en ;
	rdfs:comment "A Named Graph that has been created by selecting mappings from  another named graph into a new graph. The source graph is recorded by dcterms:source in the amalgame:provenance section."@en .

amalgame:Provenance a rdfs:Class;
	rdfs:label "Amalgame Provenance"@en ;
	rdfs:comment "Any resource that describes provenance information of graphs that are relevant for amalgame"@en .

amalgame:FullyMappedConceptScheme a rdfs:Class;
	rdfs:subClassOf skos:ConceptScheme;
	rdfs:label "100% mapped concept scheme"@en ;
	rdfs:comment "A SKOS Concept Scheme of which all concepts have been mapped to another scheme"@en .

amalgame:UnmappedConceptScheme a rdfs:Class;
	rdfs:subClassOf skos:ConceptScheme;
	rdfs:label "Unmapped concept scheme"@en ;
	rdfs:comment "A SKOS Concept Scheme of which none concepts have been mapped to another scheme"@en .

amalgame:DerivedConceptScheme a rdfs:Class;
	rdfs:subClassOf skos:ConceptScheme;
	rdfs:label "Derived concept scheme"@en ;
	rdfs:comment "A SKOS Concept Scheme which has been derived from another scheme"@en .

amalgame:member a rdf:Property ;
	rdfs:label "overlap member"@en ;
	rdfs:comment "Used to define the alignment graphs that define an OverlapMapping."@en ;
	rdfs:domain amalgame:OverlapMapping ;
	rdfs:range amalgame:Mapping .

amalgame:overlap_set
	a rdf:Property ;
	rdfs:domain amalgame:Mapping ;
	rdfs:range rdfs:Literal .

amalgame:totalCount a rdf:Property, owl:FunctionalProperty ;
	rdfs:label "total map count" ;
	rdfs:comment "The number of mappings in this Aligment" ;
	rdfs:domain amalgame:Mapping ;
	rdfs:range xsd:int .

amalgame:format a rdf:Property , owl:FunctionalProperty ;
	rdfs:label "mapping format" ;
	rdfs:comment "The format of the mappings in this Aligment, assuming a graph contains only one format." ;
	rdfs:domain amalgame:Mapping ;
	rdfs:range rdfs:Literal .

amalgame:mappedSourceConcepts a rdf:Property, owl:FunctionalProperty ;
	rdfs:domain amalgame:Mapping ;
	rdfs:range xsd:int .

amalgame:mappedTargetConcepts a rdf:Property, owl:FunctionalProperty ;
	rdfs:domain amalgame:Mapping ;
	rdfs:range xsd:int .

amalgame:nickname a rdf:Property , owl:FunctionalProperty ;
	rdfs:domain amalgame:Mapping ;
	rdfs:range rdfs:Literal .

amalgame:source a rdf:Property ;
	rdfs:subPropertyOf prov:used ;
	rdfs:range align:Ontology ;
	rdfs:range skos:ConceptScheme .

amalgame:target a rdf:Property ;
	rdfs:subPropertyOf prov:used ;
	rdfs:range align:Ontology ;
	rdfs:range skos:ConceptScheme .

amalgame:numberOfConcepts a rdf:Property , owl:FunctionalProperty ;
	rdfs:label "# Concepts"@en;
	rdfs:domain skos:ConceptScheme ;
	rdfs:range xsd:int .

amalgame:numberOfPrefLabels a rdf:Property , owl:FunctionalProperty ;
	rdfs:label "# pref. labels"@en;
	rdfs:domain skos:ConceptScheme ;
	rdfs:range xsd:int .

amalgame:numberOfAltLabels a rdf:Property , owl:FunctionalProperty ;
	rdfs:label "# alt. labels"@en;
	rdfs:domain skos:ConceptScheme ;
	rdfs:range xsd:int .

amalgame:numberOfMappedConcepts a rdf:Property , owl:FunctionalProperty ;
	rdfs:label "# mapped Concepts"@en;
	rdfs:domain skos:ConceptScheme ;
	rdfs:range xsd:int .

amalgame:provenance a rdf:Property ;
	rdfs:label "provenance informaton"@en;
	rdfs:comment "Could link to any resource describing provenance information about this alignment graph"@en ;
	rdfs:domain amalgame:Mapping ;
	rdfs:range amalgame:Provenance .

amalgame:request a rdf:Property, owl:FunctionalProperty ;
	rdfs:label "URI of the HTTP request used to create this graph"@en ;
	rdfs:domain amalgame:Provenance ;
	rdfs:range rdfs:Resource .

amalgame:sampleMethod a rdf:Property;
	rdfs:label "sample method used create this sample graph"@en ;
	rdfs:domain amalgame:Provenance ;
	rdfs:range rdfs:Literal .

amalgame:sampleSize a rdf:Property, owl:FunctionalProperty ;
	rdfs:label "sample size used create this sample graph"@en ;
	rdfs:domain amalgame:Provenance ;
	rdfs:range xsd:int .

amalgame:minimalConfidence a rdf:Property, owl:FunctionalProperty ;
	rdfs:comment "Mappings with confidence below this level have not been exported to this graph"@en ;
	rdfs:domain amalgame:Provenance ;
	rdfs:range xsd:float .

amalgame:maximalConfidence a rdf:Property, owl:FunctionalProperty ;
	rdfs:comment "Mappings with confidence above this level have not been exported to this graph"@en ;
	rdfs:domain amalgame:Provenance ;
	rdfs:range xsd:float .

amalgame:status a rdf:Property, owl:FunctionalProperty ;
        rdfs:comment "Status of a Mapping within amalgame";
	rdfs:domain amalgame:Mapping;
	rdfs:range amalgame:Status .

amalgame:Status a rdfs:Class, owl:Class ;
        owl:oneOf ( amalgame:final
		    amalgame:intermediate
		    amalgame:discarded
		    amalgame:imported ) .

amalgame:final a amalgame:Status ;
	rdfs:comment "Status indicating that a Mapping	does not need further refinement, e.g. it is of sufficient quality to be exported and used"@en .

amalgame:imported a amalgame:Status ;
	rdfs:comment "Status indicating that a Mapping has been imported into amalgame"@en .

amalgame:intermediate a amalgame:Status ;
	rdfs:comment "Status indicating that a Mapping has not insufficient quality to be useful as is, but is of potential interest as a basis for further processing."@en .

amalgame:discarded a amalgame:Status ;
	rdfs:comment "Status indicating that a Mapping has not insufficient quality to be useful, even for further processing, and can be discarded from the further analysis."@en .

amalgame:publish_ns 
	a rdf:Property ;
	rdfs:domain amalgame:AlignmentStrategy ;
	rdfs:comment "Namespace prefix to publish results of the strategy in"@en .

amalgame:default_relation
	a rdf:Property ;
	rdfs:domain amalgame:Mapping ;
	rdfs:range rdf:Property .

evaluator:unrelated
    a rdf:Property ;
    rdfs:subPropertyOf owl:differentFrom ;
    rdfs:label "unrelated"@en ;
    rdfs:comment "property used to explicitly indicate that two concepts are not related"@en .
