@prefix    align: <http://knowledgeweb.semanticweb.org/heterogeneity/alignment#> .
@prefix amalgame: <http://purl.org/vocabularies/amalgame#> .
@prefix     opmv: <http://purl.org/net/opmv/ns#> .
@prefix      owl: <http://www.w3.org/2002/07/owl#> .
@prefix      rdf: <http://www.w3.org/1999/02/22-rdf-syntax-ns#> .
@prefix     rdfs: <http://www.w3.org/2000/01/rdf-schema#> .
@prefix     skos: <http://www.w3.org/2004/02/skos/core#> .
@prefix     xsd: <http://www.w3.org/2001/XMLSchema#> .

amalgame:Process
    rdfs:label "process"@en ;
    skos:definition "Top class for all amalgame processes"@en ;
    rdfs:subClassOf opmv:Process .
amalgame:Matcher
    rdfs:label "matcher"@en ;
    skos:definition "Component that creates a mapping given a source and target vocabulary"@en ;
    rdfs:subClassOf amalgame:Process .
amalgame:Selecter
    rdfs:label "selecter"@en ;
    rdfs:subClassOf amalgame:Process .
amalgame:MultiInputComponent
    rdfs:label "multi-input operator"@en ;
    skos:definition "Component with multiple first-class inputs"@en ;
    rdfs:subClassOf amalgame:Process .
amalgame:SetOperator
    rdfs:label "set operator"@en ;
    skos:definition "Component that creates a mapping by combining the correspondences from a number of mappings"@en ;
    rdfs:subClassOf amalgame:MultiInputComponent .
amalgame:MappingSelecter
    rdfs:label "selecter"@en ;
    skos:definition "Component that creates a new mapping by selecting a number of correspondences from an existing mapping"@en ;
    rdfs:subClassOf amalgame:Selecter .
amalgame:VocabSelecter
    rdfs:label "selecter"@en ;
    skos:definition "Component that creates a new conceptScheme by selecting a number of concepts from an existing concept scheme"@en ;
    rdfs:subClassOf amalgame:Selecter .
amalgame:Subtracter
    rdfs:label "subtracter"@en ;
    skos:definition "Component that creates a new conceptScheme by subtracting a number of concepts that occur in another source"@en ;
    rdfs:subClassOf amalgame:Process .
amalgame:Merger
    rdfs:label "merger"@en ;
    skos:definition "Component that creates a mapping by mergin the correspondences from a number of mappings"@en ;
    rdfs:subClassOf amalgame:Process .


amalgame:includes
        rdfs:domain skos:ConceptScheme ;
        rdfs:range amalgame:Alignment .
amalgame:input
	rdfs:domain opmv:Process ;
	rdfs:range  amalgame:Alignment ;
	rdfs:subPropertyOf opmv:used.

amalgame:exclude
	rdfs:domain opmv:Process ;
	rdfs:range  amalgame:Alignment ;
	rdfs:subPropertyOf amalgame:secondary_input .
amalgame:secondary_input
	rdfs:domain opmv:Process ;
	rdfs:range  amalgame:Alignment ;
	rdfs:subPropertyOf opmv:used .

amalgame:wasGeneratedBy
	rdfs:subPropertyOf opmv:wasGeneratedBy.

amalgame:selectedBy
	rdfs:domain  amalgame:Alignment ;
	rdfs:range opmv:Process ;
	rdfs:subPropertyOf opmv:wasGeneratedBy.

amalgame:discardedBy
	rdfs:domain  amalgame:Alignment ;
	rdfs:range opmv:Process ;
	rdfs:subPropertyOf opmv:wasGeneratedBy.

amalgame:undecidedBy
	rdfs:domain  amalgame:Alignment ;
	rdfs:range opmv:Process ;
	rdfs:subPropertyOf opmv:wasGeneratedBy.

amalgame:evaluationOf
	rdfs:subPropertyOf opmv:wasDerivedFrom.

amalgame:NoAlignmentGraph a rdfs:Class ;
	rdfs:label "No Alignment Graph"@en ;
	rdfs:comment "The class of all Named Graphs in the repository containing no mappings and/or alignments."@en.

amalgame:Alignment a rdfs:Class ;
    rdfs:subClassOf opmv:Artifact ;
	rdfs:label "Alignment Graph"@en ;
	rdfs:comment "The class of all Named Graphs in the repository containing mappings and/or alignments."@en.

amalgame:Mapping a rdfs:Class ;
	rdfs:subClassOf amalgame:Alignment .

amalgame:LoadedMapping a rdfs:Class ;
	rdfs:subClassOf amalgame:Mapping ;
	rdfs:label "Loaded Mapping Graph"@en ;
	rdfs:comment "An alignment loaded from file, e.g. not derived from another alignment"@en.

amalgame:AmalgameAlignment a rdfs:Class ;
	rdfs:subClassOf amalgame:Alignment ;
	rdfs:label "Amalgame Alignment Graph"@en ;
	rdfs:comment "An alignment created by Amalgame's matchers, e.g. not derived from another alignment"@en.

amalgame:DerivedAlignment a rdfs:Class ;
	rdfs:subClassOf amalgame:Alignment ;
	rdfs:label "Derived Alignment Graph"@en ;
	rdfs:comment "An alignment derived from another alignment"@en.

amalgame:OverlapAlignment a rdfs:Class;
	rdfs:subClassOf amalgame:DerivedAlignment ;
	rdfs:label "Amalgame Overlap"@en ;
	rdfs:comment "A Named Graph that describes the overlap of one or more other named graphs, these constituents are denoted by the amalgame:member property."@en .

amalgame:SampleAlignment a rdfs:Class;
	rdfs:subClassOf amalgame:DerivedAlignment ;
	rdfs:label "Amalgame Sample"@en ;
	rdfs:comment "A Named Graph that describes a sample of another named graph, denoted by dcterms:source in the amalgame:provenance section."@en .

amalgame:ExportedAlignment a rdfs:Class;
	rdfs:subClassOf amalgame:DerivedAlignment ;
	rdfs:label "Amalgame Exported"@en ;
	rdfs:comment "A Named Graph that has been created by exporting another named graph into a new format. The source graph is recorded by dcterms:source in the amalgame:provenance section."@en .

amalgame:PartitionedAlignment a rdfs:Class;
	rdfs:subClassOf amalgame:DerivedAlignment ;
	rdfs:label "Amalgame Partitioned"@en ;
	rdfs:comment "A Named Graph that has been created by partitioning another named graph into one or more new graphs. The source graph is recorded by dcterms:source in the amalgame:provenance section."@en .

amalgame:EvaluatedMapping a rdfs:Class;
	rdfs:subClassOf amalgame:Mapping ;
	rdfs:label "Amalgame Evaluation Results"@en ;
	rdfs:comment "A Named Graph that has been created by manually evaluating another named graph into a new graph. The source graph is recorded by the amalgame:evaluationOf property."@en .

amalgame:SelectionAlignment a rdfs:Class;
	rdfs:subClassOf amalgame:DerivedAlignment ;
	rdfs:label "Amalgame Selection Results"@en ;
	rdfs:comment "A Named Graph that has been created by selecting mappings from  another named graph into a new graph. The source graph is recorded by dcterms:source in the amalgame:provenance section."@en .

amalgame:Provenance a rdfs:Class;
	rdfs:label "Amalgame Provenance"@en ;
	rdfs:comment "Any resource that describes provenance information of graphs that are relevant for amalgame"@en .

amalgame:FullyMappedConceptScheme a rdfs:Class;
	rdfs:subClassOf skos:ConceptScheme;
	rdfs:label "100% mapped concept scheme"@en ;
	rdfs:comment "A SKOS Concept Scheme of which all concepts have been mapped to another scheme"@en .

amalgame:UnmappedConceptScheme a rdfs:Class;
	rdfs:subClassOf skos:ConceptScheme;
	rdfs:label "Unmapped concept scheme"@en ;
	rdfs:comment "A SKOS Concept Scheme of which none concepts have been mapped to another scheme"@en .

amalgame:DerivedConceptScheme a rdfs:Class;
	rdfs:subClassOf skos:ConceptScheme;
	rdfs:label "Derived concept scheme"@en ;
	rdfs:comment "A SKOS Concept Scheme which has been derived from another scheme"@en .

amalgame:member a rdf:Property ;
	rdfs:label "overlap member"@en ;
	rdfs:comment "Used to define the alignment graphs that define an OverlapAlignment."@en ;
	rdfs:domain amalgame:OverlapAlignment ;
	rdfs:range amalgame:Alignment .

amalgame:count a rdf:Property, owl:FunctionalProperty ;
	rdfs:label "total map count" ;
	rdfs:comment "The number of mappings in this Aligment" ;
	rdfs:domain amalgame:Alignment ;
	rdfs:range xsd:int .

amalgame:format a rdf:Property , owl:FunctionalProperty ;
	rdfs:label "mapping format" ;
	rdfs:comment "The format of the mappings in this Aligment, assuming a graph contains only one format." ;
	rdfs:domain amalgame:Alignment ;
	rdfs:range rdfs:Literal .

amalgame:mappedSourceConcepts a rdf:Property, owl:FunctionalProperty ;
	rdfs:domain amalgame:Alignment ;
	rdfs:range xsd:int .

amalgame:mappedTargetConcepts a rdf:Property, owl:FunctionalProperty ;
	rdfs:domain amalgame:Alignment ;
	rdfs:range xsd:int .

amalgame:count a rdf:Property, owl:FunctionalProperty ;
	rdfs:label "total map count" ;
	rdfs:comment "The number of mappings in this Aligment" ;
	rdfs:domain amalgame:Alignment ;
	rdfs:range xsd:int .

amalgame:format a rdf:Property , owl:FunctionalProperty ;
	rdfs:label "mapping format" ;
	rdfs:comment "The format of the mappings in this Aligment, assuming a graph contains only one format." ;
	rdfs:domain amalgame:Alignment ;
	rdfs:range rdfs:Literal .

amalgame:mappedSourceConcepts a rdf:Property, owl:FunctionalProperty ;
	rdfs:domain amalgame:Alignment ;
	rdfs:range xsd:int .

amalgame:mappedTargetConcepts a rdf:Property, owl:FunctionalProperty ;
	rdfs:domain amalgame:Alignment ;
	rdfs:range xsd:int .

amalgame:nickname a rdf:Property , owl:FunctionalProperty ;
	rdfs:domain amalgame:Alignment ;
	rdfs:range rdfs:Literal .

amalgame:source a rdf:Property ;
	rdfs:subPropertyOf opmv:used ;
	rdfs:range align:Ontology ;
	rdfs:range skos:ConceptScheme .

amalgame:target a rdf:Property ;
	rdfs:subPropertyOf opmv:used ;
	rdfs:range align:Ontology ;
	rdfs:range skos:ConceptScheme .

amalgame:numberOfConcepts a rdf:Property , owl:FunctionalProperty ;
	rdfs:label "# Concepts"@en;
	rdfs:domain skos:ConceptScheme ;
	rdfs:range xsd:int .

amalgame:numberOfPrefLabels a rdf:Property , owl:FunctionalProperty ;
	rdfs:label "# pref. labels"@en;
	rdfs:domain skos:ConceptScheme ;
	rdfs:range xsd:int .

amalgame:numberOfAltLabels a rdf:Property , owl:FunctionalProperty ;
	rdfs:label "# alt. labels"@en;
	rdfs:domain skos:ConceptScheme ;
	rdfs:range xsd:int .

amalgame:numberOfMappedConcepts a rdf:Property , owl:FunctionalProperty ;
	rdfs:label "# mapped Concepts"@en;
	rdfs:domain skos:ConceptScheme ;
	rdfs:range xsd:int .

amalgame:provenance a rdf:Property ;
	rdfs:label "provenance informaton"@en;
	rdfs:comment "Could link to any resource describing provenance information about this alignment graph"@en ;
	rdfs:domain amalgame:Alignment ;
	rdfs:range amalgame:Provenance .

amalgame:request a rdf:Property, owl:FunctionalProperty ;
	rdfs:label "URI of the HTTP request used to create this graph"@en ;
	rdfs:domain amalgame:Provenance ;
	rdfs:range rdfs:Resource .

amalgame:sampleMethod a rdf:Property;
	rdfs:label "sample method used create this sample graph"@en ;
	rdfs:domain amalgame:Provenance ;
	rdfs:range rdfs:Literal .

amalgame:sampleSize a rdf:Property, owl:FunctionalProperty ;
	rdfs:label "sample size used create this sample graph"@en ;
	rdfs:domain amalgame:Provenance ;
	rdfs:range xsd:int .

amalgame:minimalConfidence a rdf:Property, owl:FunctionalProperty ;
	rdfs:comment "Mappings with confidence below this level have not been exported to this graph"@en ;
	rdfs:domain amalgame:Provenance ;
	rdfs:range xsd:float .

amalgame:maximalConfidence a rdf:Property, owl:FunctionalProperty ;
	rdfs:comment "Mappings with confidence above this level have not been exported to this graph"@en ;
	rdfs:domain amalgame:Provenance ;
	rdfs:range xsd:float .

amalgame:status a rdf:Property, owl:FunctionalProperty ;
        rdfs:comment "Status of a Mapping within amalgame";
	rdfs:domain amalgame:Mapping;
	rdfs:range amalgame:Status .

amalgame:Status a rdfs:Class, owl:Class ;
        owl:oneOf ( amalgame:final
		    amalgame:intermediate
		    amalgame:discarded
		    amalgame:imported ) .

amalgame:final a amalgame:Status ;
	rdfs:comment "Status indicating that a Mapping	does not need further refinement, e.g. it is of sufficient quality to be exported and used"@en .

amalgame:imported a amalgame:Status ;
	rdfs:comment "Status indicating that a Mapping has been imported into amalgame"@en .

amalgame:intermediate a amalgame:Status ;
	rdfs:comment "Status indicating that a Mapping has not insufficient quality to be useful as is, but is of potential interest as a basis for further processing."@en .

amalgame:discarded a amalgame:Status ;
	rdfs:comment "Status indicating that a Mapping has not insufficient quality to be useful, even for further processing, and can be discarded from the further analysis."@en .
